{
 "cells": [
  {
   "cell_type": "markdown",
   "id": "3ff3a3aa",
   "metadata": {},
   "source": [
    "# Q1- Find the value of T(2) for the recurrence relation T(n) = 3T(n-1)+12n, given that T(0) = 5."
   ]
  },
  {
   "cell_type": "code",
   "execution_count": null,
   "id": "9f51754e",
   "metadata": {},
   "outputs": [],
   "source": [
    "T(n) = 3T(n-1)+12n ---->(1)\n",
    "T(n-1) = 3T(n-2)+12(n-1) ---->(2)\n",
    "substituting the value of (2) in (1), we get\n",
    "T(n) = 3(3T(n-2)+12(n-1))+12n\n",
    "putting n = 2,\n",
    "T(2) = 3(3T(0)+12(1))+12(2)\n",
    "T(2) = 3(3*5+12)+24 ..........(since T(0)=5)\n",
    "T(2) = 81+24\n",
    "T(2) = 105\n",
    "\n",
    "Therefore, the value of T(2) for the given recurrence relation and initial condition is 105"
   ]
  },
  {
   "cell_type": "markdown",
   "id": "dfc05170",
   "metadata": {},
   "source": [
    "# 2. Given a recurrence relation, solve it using the substitution method:"
   ]
  },
  {
   "cell_type": "code",
   "execution_count": null,
   "id": "bd045a88",
   "metadata": {},
   "outputs": [],
   "source": [
    "a. T(n) = T(n-1) + c\n",
    "\n",
    "The recurrence relation is given as:\n",
    "\n",
    "T(n) = T(n-1) + c\n",
    "\n",
    "We can start by expanding this relation:\n",
    "\n",
    "T(n) = T(n-1) + c = T(n-2) + c + c = T(n-3) + c + c + c \n",
    "\n",
    "Continuing this process, we get:\n",
    "\n",
    "T(n) = T(n-k) + kc\n",
    "\n",
    "We know that the base case is T(1), so n-1=k  ,k=n-1, and substituting this in we get:\n",
    "\n",
    "T(n) = T(1) + c(n-1)\n",
    "\n",
    "So, the solution to the given recurrence relation is T(n) = T(1) + c(n-1).\n"
   ]
  },
  {
   "cell_type": "code",
   "execution_count": null,
   "id": "ffdcd1f4",
   "metadata": {},
   "outputs": [],
   "source": [
    "b. T(n) = 2T(n/2) + n\n",
    "\n",
    "The recurrence relation is given as:\n",
    "\n",
    "T(n) = 2T(n/2) + n\n",
    "\n",
    "We can start by expanding this relation:\n",
    "\n",
    "T(n) = 2T(n/2) + n = 2[2T(n/4) + n/2] + n = 2^2T(n/2^2) + 2n\n",
    "\n",
    "Continuing this process, we get:\n",
    "\n",
    "T(n) = 2^kT(n/2^k) + kn\n",
    "\n",
    "We know that the base case is T(1), so n/2^k=1 => k=log_2{n}, and substituting this in we get:\n",
    "\n",
    "T(n) = nT(1) + nlog_2{n}\n",
    "\n",
    "So, the solution to the given recurrence relation is T(n) = nT(1) + nlog_2{n}. "
   ]
  },
  {
   "cell_type": "code",
   "execution_count": null,
   "id": "c5eb6fe1",
   "metadata": {},
   "outputs": [],
   "source": [
    "c.T(n) = 2T(n/2) + c\n",
    "\n",
    "The recurrence relation is given as:\n",
    "\n",
    "T(n) = 2T(n/2) + c\n",
    "\n",
    "We can start by expanding this relation:\n",
    "\n",
    "T(n) = 2T(n/2) + c = 2[2T(n/4) + c] + c = 2^2T(n/2^2) + 2c\n",
    "\n",
    "Continuing this process, we get:\n",
    "\n",
    "T(n) = 2^kT(n/2^k) + kc\n",
    "\n",
    "We know that the base case is T(1), so n/2^k=1 => k=log_2{n}, and substituting this in we get:\n",
    "\n",
    "T(n) = T(1) + clog_2{n}\n",
    "\n",
    "So, the solution to the given recurrence relation is $T(n) = T(1) + clog_2{n}. "
   ]
  },
  {
   "cell_type": "code",
   "execution_count": null,
   "id": "8022a4a1",
   "metadata": {},
   "outputs": [],
   "source": [
    "d.T(n)=T(n/2)+c\n",
    "\n",
    "The recurrence relation is given as:\n",
    "\n",
    "T(n) = T(n/2) + c\n",
    "\n",
    "We can start by expanding this relation:\n",
    "\n",
    "T(n) = T(n/2) + c = T(n/4) + c + c = T(n/8) + c + c + c \n",
    "\n",
    "Continuing this process, we get:\n",
    "\n",
    "T(n) = T(n/2^k) + kc\n",
    "\n",
    "We know that the base case is T(1), so n/2^k=1 => k=log_2{n}, and substituting this in we get:\n",
    "\n",
    "T(n) = T(1) + clog_2{n}\n",
    "\n",
    "So, the solution to the given recurrence relation is T(n) = T(1) + clog_2{n}. "
   ]
  },
  {
   "cell_type": "markdown",
   "id": "4df4e88e",
   "metadata": {},
   "source": [
    "# 3. Given a recurrence relation, solve it using the recursive tree approach:"
   ]
  },
  {
   "cell_type": "code",
   "execution_count": null,
   "id": "d422aa55",
   "metadata": {},
   "outputs": [],
   "source": [
    "a. T(n) = 2T(n-1) +1\n",
    "\n",
    "To solve the given recurrence relation T(n) = 2T(n-1) + 1 using the recursive tree approach, we can visualize the recursion as a tree. Each node in the tree represents a subproblem, and the edges represent the recursive calls. Here's how the recursive tree looks for this recurrence relation:\n",
    "\n",
    "\n",
    "      T(n)\n",
    "      /  \\\n",
    "  T(n-1)  T(n-1)\n",
    "   / \\      / \\\n",
    "T(n-2) T(n-2) ...\n",
    "  / \\      / \\\n",
    "...  ...  ... ...\n",
    "\n",
    "\n",
    "At each level of the tree, the problem size decreases by 1, and each node has two children corresponding to the recursive calls with (n-1) as the argument.\n",
    "\n",
    "Now, let's write down the recursive relation for the tree:\n",
    "\n",
    "\n",
    "T(n) = 2T(n-1) + 1\n",
    "\n",
    "\n",
    "T(n-1) = 2T(n-2) + 1\n",
    "\n",
    "T(n-2) = 2T(n-3) + 1\n",
    "\n",
    "\n",
    "T(2) = 2T(1) + 1\n",
    "\n",
    "Now, let's substitute these relations back into the original one:\n",
    "\n",
    "T(n) = 2[2T(n-2) + 1] + 1\n",
    "\n",
    "\n",
    "\n",
    "T(n) = 2^2T(n-2) + 2 + 1\n",
    "\n",
    "\n",
    "Similarly,\n",
    "\n",
    "\n",
    "T(n) = 2^3T(n-3) + 2^2 + 2 + 1\n",
    "\n",
    "\n",
    "Continuing this pattern, we get:\n",
    "\n",
    "\n",
    "T(n) = 2^kT(n-k) + 2^{k-1} + 2^{k-2} + .... + 2^2 + 2 + 1\n",
    "\n",
    "\n",
    "Now, we know that the base case is (T(1)), so when (n-k = 1), we have (k = n-1). Substituting this back:\n",
    "\n",
    "\n",
    "T(n) = 2^{n-1}T(1) + 2^{n-2} + 2^{n-3} + .... + 2^2 + 2 + 1\n",
    "\n",
    "\n",
    "Finally, we can simplify this using the geometric series formula:\n",
    "\n",
    "T(n) = 2^{n-1}T(1) + 2^{n-1} - 1\n",
    "\n",
    "So, the solution to the given recurrence relation using the recursive tree approach is T(n) = 2^{n-1}T(1) + 2^{n-1} - 1."
   ]
  },
  {
   "cell_type": "code",
   "execution_count": null,
   "id": "b04d02c0",
   "metadata": {},
   "outputs": [],
   "source": [
    "b. T(n) = 2T(n/2) + n\n",
    "\n",
    "To solve the given recurrence relation T(n) = 2T(n/2) + n using the recursive tree approach, we can visualize the recursion as a tree. Each node in the tree represents a subproblem, and the edges represent the recursive calls. Here's how the recursive tree looks for this recurrence relation:\n",
    "\n",
    "\n",
    "         T(n)\n",
    "        /   \\\n",
    "   T(n/2)   T(n/2)\n",
    "   /   \\    /   \\\n",
    "T(n/4) ... T(n/4)  (and so on)\n",
    "\n",
    "\n",
    "At each level of the tree, the problem size decreases by a factor of 2, and each node has two children corresponding to the recursive calls with (n/2) as the argument.\n",
    "\n",
    "Now, let's write down the recursive relation for the tree:\n",
    "\n",
    "\n",
    "T(n) = 2T(n/2) + n\n",
    "\n",
    "T(n/2) = 2T(n/4) + n/2\n",
    "\n",
    "T(n/4) = 2T(n/8) + n/4\n",
    "\n",
    ".\n",
    ".\n",
    ".\n",
    "\n",
    "T(2) = 2T(1) + 2\n",
    "\n",
    "\n",
    "Now, let's substitute these relations back into the original one:\n",
    "\n",
    "\n",
    "T(n) = 2[2T(n/2)+n/2] + n\n",
    "\n",
    "\n",
    "T(n) = 2^2T(n/2) + 2n\n",
    "\n",
    "\n",
    "Similarly,\n",
    "\n",
    "T(n) = 2^3T(n/4) + 3n\n",
    "\n",
    "\n",
    "Continuing this pattern, we get:\n",
    "\n",
    "T(n) = 2^kT(n/2^k) + kn\n",
    "\n",
    "\n",
    "Now, we know that the base case is (T(1)), so when n/2^k =1, we have k = log_2{n}. Substituting this back:\n",
    "\n",
    "\n",
    "T(n) = 2^{log_2{n}}T(1) + nlog_2{n}\n",
    "\n",
    "\n",
    "Simplifying using (2^{log_2{n}} = n):\n",
    "\n",
    "\n",
    "T(n) = nT(1) + nlog_2{n}\n",
    "\n",
    "\n",
    "So, the solution to the given recurrence relation using the recursive tree approach is T(n) = nT(1) + nlog_2{n}."
   ]
  }
 ],
 "metadata": {
  "kernelspec": {
   "display_name": "Python 3 (ipykernel)",
   "language": "python",
   "name": "python3"
  },
  "language_info": {
   "codemirror_mode": {
    "name": "ipython",
    "version": 3
   },
   "file_extension": ".py",
   "mimetype": "text/x-python",
   "name": "python",
   "nbconvert_exporter": "python",
   "pygments_lexer": "ipython3",
   "version": "3.9.13"
  }
 },
 "nbformat": 4,
 "nbformat_minor": 5
}
